test-suite/f91.v
@@ -11,40 +11,54 @@ Require Import Equations Bvector List.
 Require Import Relations.
 Require Import DepElimDec.
 Require Import Subterm.
-
+Require Import Omega.
 Require Import Arith Wf_nat.
+
 Instance wf_nat : WellFounded lt := lt_wf.
 Hint Resolve lt_n_Sn : Below.
-Ltac rec ::= rec_wf_eqns.
-
-Definition measure {A B} (f : A -> B) (R : relation B) : relation A :=
-  fun x y => R (f x) (f y).
 
 Definition f91_rel : relation nat :=
-  measure (fun x => 101 - x) lt.
+  MR lt (fun x => 101 - x).
 
 Instance gt_bound_wf : WellFounded f91_rel.
-Proof. red. red. intros.
-Admitted.
+Proof. red. unfold f91_rel. apply measure_wf. apply lt_wf. Defined.
+Lemma f91_1 n : n <= 100 -> f91_rel (n + 11) n.
+Proof. intros.
+  - do 2 red; abstract omega.
+Qed.
+
+Lemma f91_2 :   forall (n : nat) (H : n <= 100)
+    (f91 : forall x : nat, f91_rel x n -> {m : nat | if le_lt_dec x 100 then m = 91 else m = x - 10}),
+  f91_rel (` (f91 (n + 11) (f91_1 n H))) n.
+Proof.
+  intros.
+  - do 2 red; destruct f91; cbn [proj1_sig];
+    destruct le_lt_dec; subst; abstract omega.
+Defined.
 
 Set Program Mode.
-Equations f91 n : { m : nat | if le_lt_dec n 100 then m = 91 else m = n - 10 } by rec n f91_rel :=
+Equations? f91 n : { m : nat | if le_lt_dec n 100 then m = 91 else m = n - 10 } by rec n f91_rel :=
 f91 n with le_lt_dec n 100 := {
   | left H := f91 (f91 (n + 11)) ;
   | right H := (n - 10) }.
-
-Require Import Omega.
-
-Next Obligation. intros. do 2 red. try omega. Defined.
-Next Obligation. intros. destruct f91. simpl. do 2 red.
-  destruct_call le_lt_dec. subst. omega. subst. omega.
+Proof.
+  - apply (f91_1 _ H).
+  - apply f91_2.
+  - unfold f91_2. destruct f91; cbn [proj1_sig];
+    destruct f91; cbn [proj1_sig];
+    destruct le_lt_dec; subst; simpl in y0; auto;
+    destruct le_lt_dec; subst; auto; omega.
 Defined.
 
-Next Obligation. destruct_call f91; simpl.
-  destruct_call f91. simpl in *. destruct le_lt_dec. subst. simpl in y. auto.
-  subst x0. destruct le_lt_dec; auto.
-  subst x. simpl. omega.
-Defined.
+(* Next Obligation. intros. destruct f91. simpl. do 2 red. *)
+(*   destruct_call le_lt_dec. subst. omega. subst. omega. *)
+(* Defined. *)
+
+(* Next Obligation. destruct_call f91; simpl. *)
+(*   destruct_call f91. simpl in *. destruct le_lt_dec. subst. simpl in y. auto. *)
+(*   subst x0. destruct le_lt_dec; auto. *)
+(*   subst x. simpl. omega. *)
+(* Defined. *)
 
 (** MS: Bug, this should be derivable, but needs the user's proofs as hints (omega calls) *)
 Next Obligation.
@@ -54,7 +68,6 @@ Next Obligation.
   do 2 red; omega.
   apply IH. do 2 red. destruct_call f91. simpl proj1_sig.
   destruct le_lt_dec; subst; repeat red; omega.
-  constructor.
+  intros. apply IH. auto.
+  simp f91.
 Defined.
-
-Notation "( x &?) " := (exist _ x _).
