test-suite/nestedwfrec.v
@@ -1,9 +1,9 @@
-Require Import Equations.Equations.
+From Equations Require Import Equations.
 Require Import Lia.
 
 Set Equations Debug.
 
-Equations f (n : nat) : nat by rec n lt :=
+Equations?(noind) f (n : nat) : nat by rec n lt :=
   f 0 := 0;
   f (S k) := g k (le_n (S k))
 
@@ -12,7 +12,11 @@ Equations f (n : nat) : nat by rec n lt :=
   g (S n') H := f n' + g n' (PeanoNat.Nat.lt_le_incl (S n') (S k) H).
 
 Hint Extern 0 (_ < _) => lia : f.
-Next Obligation. lia. Qed.
+Proof. lia. Defined.
+                                  ============================
+                                  forall (k n' : nat) (H : n' < S k)
+                                    (g : forall x : nat, x < S k -> x < n' -> nat),
+                                  f_clause_2_g n' H g = f_unfold_clause_2_g k n' H g
 
 Goal f 2 = 1.
 Proof. reflexivity. Defined.
